pcuic/theories/PCUICReduction.v
@@ -1,0 +1,231 @@
+(* Distributed under the terms of the MIT license.   *)
+From Equations Require Import Equations.
+From Coq Require Import Bool String List Program BinPos Compare_dec Omega.
+From Template Require Import config utils univ BasicAst.
+From PCUIC Require Import PCUICAst PCUICAstUtils PCUICInduction
+     PCUICLiftSubst PCUICUnivSubst PCUICTyping PCUICWeakeningEnv PCUICWeakening
+     PCUICSubstitution PCUICClosed.
+Require Import ssreflect ssrbool.
+Require Import String.
+Require Import LibHypsNaming.
+Local Open Scope string_scope.
+Set Asymmetric Patterns.
+
+Existing Instance config.default_checker_flags.
+
+Lemma red_step Σ Γ t u v : red1 Σ Γ t u -> red Σ Γ u v -> red Σ Γ t v.
+Proof.
+  induction 2. econstructor; auto. constructor. apply X.
+  econstructor 2; eauto.
+Qed.
+
+Require Import Equations.Type.Relation Equations.Type.Relation_Properties.
+
+Lemma red_alt@{i j +} Σ Γ t u : red Σ Γ t u <~> clos_refl_trans@{i j} (red1 Σ Γ) t u.
+Proof.
+  split. intros H. apply clos_rt_rtn1_iff.
+  induction H; econstructor; eauto.
+  intros H. apply clos_rt_rtn1_iff in H.
+  induction H; econstructor; eauto.
+Qed.
+
+(** Atoms do not reduce *)
+
+Definition atom t :=
+  match t with
+  | tVar _
+  | tMeta _
+  | tSort _
+  | tInd _ _
+  | tConstruct _ _ _ => true
+  | _ => false
+  end.
+
+Section ParallelReduction.
+  Context (Σ : global_declarations).
+
+  Inductive pred1 (Γ : context) : term -> term -> Type :=
+  (** Reductions *)
+  (** Beta *)
+  | pred_beta na t b0 b1 a0 a1 :
+      pred1 Γ b0 b1 -> pred1 Γ a0 a1 ->
+      pred1 Γ (tApp (tLambda na t b0) a0) (subst10 a1 b1)
+
+  (** Let *)
+  | pred_zeta na d0 d1 t b0 b1 :
+      pred1 Γ d0 d1 -> pred1 Γ b0 b1 ->
+      pred1 Γ (tLetIn na d0 t b0) (subst10 d1 b1)
+
+  (** Local variables *)
+  | pred_rel_def i body body' :
+      option_map decl_body (nth_error Γ i) = Some (Some body) ->
+      pred1 Γ (lift0 (S i) body) body' ->
+      pred1 Γ (tRel i) body'
+
+  | pred_rel_assum i :
+      option_map decl_body (nth_error Γ i) = Some None ->
+      pred1 Γ (tRel i) (tRel i)
+
+  (** Case *)
+  | pred_iota ind pars c u args0 args1 p brs0 brs1 :
+      All2 (pred1 Γ) args0 args1 ->
+      All2 (on_Trel (pred1 Γ) snd) brs0 brs1 ->
+      pred1 Γ (tCase (ind, pars) p (mkApps (tConstruct ind c u) args0) brs0)
+            (iota_red pars c args1 brs1)
+
+  (** Fix unfolding, with guard *)
+  | pred_fix mfix idx args0 args1 narg fn0 fn1 :
+      unfold_fix mfix idx = Some (narg, fn0) ->
+      is_constructor narg args1 = true ->
+      All2 (pred1 Γ) args0 args1 ->
+      pred1 Γ fn0 fn1 ->
+      pred1 Γ (mkApps (tFix mfix idx) args0) (mkApps fn1 args1)
+
+  (** CoFix-case unfolding *)
+  | pred_cofix_case ip p0 p1 mfix idx args0 args1 narg fn0 fn1 brs0 brs1 :
+      unfold_cofix mfix idx = Some (narg, fn0) ->
+      All2 (pred1 Γ) args0 args1 ->
+      pred1 Γ fn0 fn1 ->
+      pred1 Γ p0 p1 ->
+      All2 (on_Trel (pred1 Γ) snd) brs0 brs1 ->
+      pred1 Γ (tCase ip p0 (mkApps (tCoFix mfix idx) args0) brs0)
+            (tCase ip (mkApps fn1 args1) p1 brs1)
+
+  (** CoFix-proj unfolding *)
+  | pred_cofix_proj p mfix idx args0 args1 narg fn0 fn1 :
+      unfold_cofix mfix idx = Some (narg, fn0) ->
+      All2 (pred1 Γ) args0 args1 ->
+      pred1 Γ fn0 fn1 ->
+      pred1 Γ (tProj p (mkApps (tCoFix mfix idx) args0))
+            (tProj p (mkApps fn1 args1))
+
+  (** Constant unfolding *)
+
+  | pred_delta c decl body (isdecl : declared_constant Σ c decl) u :
+      decl.(cst_body) = Some body ->
+      pred1 Γ (tConst c u) (subst_instance_constr u body)
+
+  | pred_axiom c decl (isdecl : declared_constant Σ c decl) u :
+      decl.(cst_body) = None ->
+      pred1 Γ (tConst c u) (tConst c u)
+
+  (** Proj *)
+  | pred_proj i pars narg args k u args0 args1 arg1 :
+      All2 (pred1 Γ) args0 args1 ->
+      nth_error args (pars + narg) = Some arg1 ->
+      pred1 Γ (tProj (i, pars, narg) (mkApps (tConstruct i k u) args0)) arg1
+
+  (** Congruences *)
+  | pred_abs na M M' N N' : pred1 Γ M M' -> pred1 (Γ ,, vass na M) N N' ->
+                            pred1 Γ (tLambda na M N) (tLambda na M' N')
+  | pred_app M0 M1 N0 N1 :
+      pred1 Γ M0 M1 ->
+      pred1 Γ N0 N1 ->
+      pred1 Γ (tApp M0 N0) (tApp M1 N1)
+            (* do not handle mkApps yet *)
+  | pred_letin na d0 d1 t0 t1 b0 b1 :
+      pred1 Γ d0 d1 -> pred1 Γ t0 t1 -> pred1 (Γ ,, vdef na d0 t0) b0 b1 ->
+      pred1 Γ (tLetIn na d0 t0 b0) (tLetIn na d1 t1 b1)
+
+  | pred_case ind p0 p1 c0 c1 brs0 brs1 :
+      pred1 Γ p0 p1 ->
+      pred1 Γ c0 c1 ->
+      All2 (on_Trel (pred1 Γ) snd) brs0 brs1 ->
+      pred1 Γ (tCase ind p0 c0 brs0) (tCase ind p1 c1 brs1)
+
+  | pred_proj_congr p c c' : pred1 Γ c c' -> pred1 Γ (tProj p c) (tProj p c')
+
+  | pred_fix_congr mfix0 mfix1 idx :
+      All2 (fun d0 d1 => (pred1 Γ (dtype d0) (dtype d1)) *
+                         (pred1 (Γ ,,, fix_context mfix0) (dbody d0) (dbody d1)))%type mfix0 mfix1 ->
+      pred1 Γ (tFix mfix0 idx) (tFix mfix1 idx)
+
+  | pred_cofix_congr mfix0 mfix1 idx :
+      All2 (fun d0 d1 => (pred1 Γ (dtype d0) (dtype d1)) *
+                            (pred1 (Γ ,,, fix_context mfix0) (dbody d0) (dbody d1)))%type mfix0 mfix1 ->
+      pred1 Γ (tCoFix mfix0 idx) (tCoFix mfix1 idx)
+
+  | pred_prod na M0 M1 N0 N1 : pred1 Γ M0 M1 -> pred1 (Γ ,, vass na M0) N0 N1 ->
+                               pred1 Γ (tProd na M0 N0) (tProd na M1 N1)
+
+  | evar_pred ev l l' : All2 (pred1 Γ) l l' -> pred1 Γ (tEvar ev l) (tEvar ev l')
+
+  | pred_atom t : atom t -> pred1 Γ t t.
+
+  Lemma pred1_refl Γ t : pred1 Γ t t.
+  Proof.
+    induction t in Γ |- * using term_forall_list_ind;
+      try solve [(apply pred_atom; reflexivity) || constructor; auto].
+    constructor. solve_all; eapply All_Forall2; eauto. simpl. auto.
+    econstructor; auto. solve_all. eapply All_Forall2; eauto. simpl; auto.
+    constructor; eauto. red in H. solve_all. eapply All_Forall2; eauto. simpl; intuition auto.
+    red. auto.
+    constructor; eauto. red in H. solve_all. eapply All_Forall2; eauto. simpl; intuition auto.
+    constructor; eauto. red in H. solve_all. eapply All_Forall2; eauto. simpl; intuition auto.
+  Qed.
+
+  Hint Constructors pred1 : pred.
+  Hint Resolve pred1_refl : pred.
+
+  Lemma Forall2_same {A} (P : A -> A -> Prop) l : (forall x, P x x) -> Forall2 P l l.
+  Proof. induction l; constructor; auto. Qed.
+
+  Hint Resolve Forall2_same : pred.
+  Hint Unfold on_rel snd on_snd : pred.
+
+  Lemma red1_pred1 Γ : forall M N, red1 Σ Γ M N -> pred1 Γ M N.
+    induction 1 using red1_ind_all; intros; eauto with pred.
+
+    constructor; auto with pred.
+    induction H. intuition. constructor; auto with pred.
+    admit.
+
+    constructor. auto with pred.
+    induction H. constructor; intuition auto with pred.
+    constructor; auto with pred.
+    constructor; auto with pred.
+
+    induction H; constructor; intuition auto with pred.
+
+    constructor.
+    generalize (fix_context mfix0).
+    induction H; constructor; intuition auto with pred.
+    rewrite H1; auto with pred.
+
+    constructor.
+    revert H.
+    generalize (fix_context mfix0).
+    induction 1; constructor; intuition auto with pred.
+    rewrite H1; auto with pred.
+
+    constructor.
+    generalize (fix_context mfix0).
+    induction H; constructor; intuition auto with pred.
+    rewrite H1; auto with pred.
+
+    constructor.
+    revert H.
+    generalize (fix_context mfix0).
+    induction 1; constructor; intuition auto with pred.
+    rewrite H1; auto with pred.
+  Admitted.
+
+  Lemma pred1_red Γ : forall M N, pred1 Γ M N -> red Σ Γ M N.
+  Proof.
+    induction 1; try constructor; auto with pred.
+  Admitted.
+
+End ParallelReduction.
+
+Lemma substitution_pred1 `{cf:checker_flags} Σ Γ Γ' Γ'' s M N :
+  wf Σ -> All Ast.wf s -> subs Σ Γ s Γ' -> wf_local Σ Γ -> Ast.wf M ->
+  wf_local Σ (Γ ,,, Γ' ,,, Γ'') ->
+  pred1 (fst Σ) (Γ ,,, Γ' ,,, Γ'') M N ->
+  pred1 (fst Σ) (Γ ,,, subst_context s 0 Γ'') (subst s #|Γ''| M) (subst s #|Γ''| N).
+Proof.
+  intros.
+  induction H1. constructor.
+  econstructor 2; eauto.
+  eapply substitution_red1; eauto.
+  eapply wf_red_wf. 4:eauto. all:eauto.
+Qed.
